<chapter xmlns:xi="http://www.w3.org/2001/XInclude"  xml:id="Interegnum">
  <title>Joseph Fourier: The Man Who Broke Calculus</title>
  <section><title>Joseph Fourier and His Series</title>
  <p>
    Applying mathematics to physical problems such as heat flow in a
    solid body drew much attention in the latter part of the 1700<rsq/>s
    and the early part of the 1800<rsq/>s.  One of the people to attack the
    heat flow problem was <url
    href="https://mathshistory.st-andrews.ac.uk/Biographies/Fourier/"
    >Jean
    Baptiste Joseph Fourier</url> (1768<ndash/>1839).
  </p>

  <figure>
    <caption>  Jean Baptiste Joseph Fourier  </caption>

    <idx><h>Fourier, Jean Baptiste Joseph</h><h>portrait of</h></idx>
    <idx><h>Portraits</h><h>Fourier</h></idx>

    <image width="35%" source="images/Fourier.png" >
      <shortdescription></shortdescription>
    </image>
  </figure>

  <p>
    <idx><h>Fourier, Jean Baptiste Joseph</h></idx>

    Fourier submitted a manuscript on the subject, <foreign>Sur la
    propagation de la chaleur</foreign> (<pubtitle>On the Propagation of
    Heat</pubtitle>), to the <foreign>Institut National des Sciences et des
    Arts</foreign> in 1807.  These ideas were subsequently published
    in <foreign>La theorie analytique de la chaleur</foreign> (<pubtitle>The
    Analytic Theory of Heat (1822)</pubtitle>).
  </p>

  <p>
    To examine Fourier<rsq/>s ideas, consider the example of a thin
    wire of length one, which is perfectly insulated and whose
    endpoints are held at a fixed temperature of zero.  Given an
    initial temperature distribution in the wire, the problem is to
    monitor the temperature of the wire at any point <m>x</m> and at
    any time <m>t</m>.  Specifically, if we let <m>u(x,t)</m> denote
    the temperature of the wire at point <m>x\in[0,1]</m> at time
    <m>t\geq 0</m>, then it can be shown that <m>u</m> must satisfy
    the one-dimensional heat equation
    <m>\rho^2\frac{\partial^2u}{\partial x^2}=\frac{\partial
    u}{\partial t}</m>, where <m>\rho^2</m> is a positive constant
    known as the <term>thermal diffusivity</term>.  If the initial
    temperature distribution is given by the function <m>f(x)</m>,
    then the <m>u</m> we are seeking must satisfy all of the following.

    <mdn>

      <mrow xml:id="EQUATIONHeatEquation">
        \rho^2\frac{\partial^2u}{\partial x^2}\amp{}=\frac{\partial u}{\partial t},\amp{}
      </mrow>
      <mrow number="no">
        
        u(0,t)\amp{} =u(1,t)=0,  
        \amp{}
        \forall\  t\amp{}\geq 0,
      </mrow>
      <mrow number="no">
        u(x,0)\amp{} =f(x), 
        \amp{}
        \forall\  x\amp{}\in[\,0,1].
      </mrow>

    </mdn>

  </p>

  <p>
    To do this, Fourier employed what is now referred to as the method
    of separation of variables.  Specifically, Fourier looked for
    solutions of the form <m>u(x,t)=X(x)T(t)</m>; that is, solutions
    where the <m>x</m><ndash/>part can be separated from the <m>t</m>-part.
    Assuming that <m>u</m> has this form, we get
    <m>\frac{\partial^2u}{\partial x^2}=X^{\prime\prime}T</m> and
    <m>\frac{\partial u}{\partial t}=X\,T^{\prime}</m>.  Substituting
    these into <xref ref="EQUATIONHeatEquation">equation</xref> we
    obtain

    <md>
      <mrow>
        \rho^2X^{\prime\prime}T=X
        T^\prime\amp{}\amp{}\text{or}\amp{}\amp{}
        \frac{X^{\prime\prime}}{X}=\frac{T^\prime}{\rho^2T}
      </mrow>
      </md>.
  </p>

  <p>
    Since the left-hand side involves no <m>t</m><rsq/>s and the
    right-hand side involves no <m>x</m><rsq/>s, both sides must equal
    a constant <m>k</m>.  Thus we have

    <md>

      <mrow>
        X^{\prime\prime}=k X\amp{}\amp{}\text{and}\amp{}\amp{}
        T^\prime=\rho^2k T.
      </mrow>

    </md>

  </p>

  <problem xml:id="prob_HarmonicMotion">

    <idx><h>Heat Equation, the</h></idx> 
    <idx><h>Heat Equation, the</h><h>parameter <m>k</m> must be less
    than zero</h></idx>

    <statement>
    <p>
      Show that <m>T=Ce^{\rho^2kt}</m> satisfies the equation
      <m>T^\prime=\rho^2k T</m>, where <m>C</m> is an arbitrary
      constant.  Use the physics of the problem to show that if
      <m>u</m> is not constantly zero, then <m>k\lt 0</m>.
    </p>
    </statement>
    <hint>
      <p>
        Consider <m>\limit{t}{\infty}{u(x,t)}</m>.
      </p>
    </hint>
  </problem>

  <p>
    Using the reslut from <xref ref="prob_HarmonicMotion"></xref> that <m>k\lt 0</m>,
    we will let <m>k=-p^2</m>.
  </p>

  <problem>

    <idx><h>Heat Equation, the</h></idx>
    <idx><h>Heat Equation, the</h><h>solving for <m>\xi(x)</m></h></idx>
    
    <statement>
      <p>
        Show that <m>X=A\sin\left(px\right)+B\cos\left(px\right)</m>
        satisfies the equation <m>X^{\prime\prime}=-p^2X</m>, where <m>A</m> and
        <m>B</m> are arbitrary constants.  Use the boundary conditions
        <m>u(0,t)=u(1,t)=0</m>, <m>\forall</m> <m>t\geq 0</m> to show that
        <m>B=0</m> and <m>A\sin p=0</m>.  Conclude that if <m>u</m> is
        not constantly zero, then <m>p=n\pi</m>, where <m>n</m> is any
        integer.
      </p>
    </statement>
  </problem>

  <problem>
    
    <idx><h>Heat Equation, the</h><h>fundamental solutions of</h></idx>

    <statement>
      <p>
        Show that if <m>u_1</m> and <m>u_2</m> satisfy the equations
        <me>
          \rho^2\frac{\partial^2u}{\partial x^2}=\frac{\partial
        u}{\partial t}
        </me>
        and 

        <md>
          <mrow>
            u(0,t)=u(1,t)=0,\amp{}\amp{} \forall\  t\geq   0
          </mrow> 

        </md>

          then <m>u=A_1u_1+A_2u_2</m> satisfy them as well, where
          <m>A_1</m> and <m>A_2</m> are arbitrary constants.
      </p>
    </statement>
  </problem>

  <p>
    
    <idx><h>Fourier, Jean Baptiste Joseph</h></idx>

    Putting all of these results together, Fourier surmised that the general solution to

    <md>
      <mrow>
        \rho^2\frac{\partial^2u}{\partial x^2}=\frac{\partial
          u}{\partial t} u(0,t)=u(1,t)=0,\amp{}\amp{}\forall\ t\geq 0
      </mrow>

    </md>
    could be expressed as the series
    <me>
      u(x,t)=\sum_{n=1}^\infty A_ne^{-(\rho n\pi)^2t}\sin\left(n\pi x\right)
      </me>.
  </p>

  <p>
    All that is left is to have <m>u</m> satisfy the initial condition <m>u(x,0)=f(x)</m>,
    <m>\forall\,x\in[\,0,1]</m>.
    That is, we need to find coefficients <m>A_n</m>, such that
    <me>
      f(x)=u(x,0)=\sum_{n=1}^\infty A_n\sin\left(n\pi x\right)
      </me>.
  </p>

  <p>
    The idea of representing a function as a series of sine waves was proposed by Daniel Bernoulli in 1753 while examining the problem of modeling a vibrating string.
    Unfortunately for Bernoulli,
    he didn<rsq/>t know how to compute the coefficients in such a series representation.
    What distinguished Fourier was that he developed a technique to compute these coefficients.
    The key is the result of the following problem.
  </p>

  <problem xml:id="prob_SinOrthogonality">
    <idx><h><m>\sin x</m></h><h>orthogonality of</h></idx>
    <idx><h>orthogonality</h><h> of <m>\sin nx</m></h></idx>
    <statement>
      <p>
        Let <m>n</m> and <m>m</m> be positive integers.
        Show
        <me>
          \int_{x=0}^1\sin\left(n\pi x\right)\sin\left(m\pi x\right)\dx{ x}= \left\{\begin{matrix}0\amp \text{ if } n\neq m\\ \frac{1}{2}\amp \text{ if } n=m \end{matrix} \right.. {}
        </me>
      </p>
    </statement>
  </problem>

  <p>
    <idx><h>Fourier, Jean Baptiste Joseph</h></idx>

    Armed with the result from <xref
    ref="prob_SinOrthogonality"></xref>, Fourier could compute the
    coefficients <m>A_n</m> in the series representation
    <m>f(x)=\sum_{n=1}^\infty A_n \sin\left(n\pi x\right)</m> in the
    following manner.  Since we are trying to find <m>A_n</m> for a
    particular (albeit general) <m>n</m>, we will temporarily change
    the index in the summation from <m>n</m> to <m>j</m>.  With this
    in mind, consider
    <md>
      <mrow>\int_{x=0}^1f(x)\sin\left(n\pi x\right)\dx{ x} \amp =\int_{x=0}^1\left(\sum_{j=1}^\infty A_j\text{ sin } \left(j\pi x\right)\right)\sin\left(n\pi x\right)\dx{ x}</mrow>
      <mrow>\amp =\sum_{j=1}^\infty A_j\int_{x=0}^1\sin\left(j\pi x\right)\sin\left(n\pi x\right)\dx{ x}</mrow>
      <mrow>\amp =\frac{A_n}{2}</mrow>
    </md>
    which leads to the formula <m>A_n=2\int_{x=0}^1f(x)\sin\left(n\pi x\right)d x</m>.
  </p>

    <p>
      The series <m>f(x)=\sum_{n=1}^\infty A_n\sin\left(n\pi
      x\right)</m> with
      <men xml:id="EQUATIONSineCoeffFourier">
        A_n=2\int_{x=0}^1f(x)\sin\left(n\pi
        x\right)\dx{ x}
      </men> 
      is called the <term>Fourier (sine) series of
      <m>\boldsymbol{f}</m></term>.
    </p>

    <example>
      <statement>
        <p>
          Let<rsq/>s apply this to the function,
          <m>f(x)=\frac{1}{2}-\abs{x-\frac{1}{2}}</m>, whose graph is
          seen below.
        </p>
        <image width="75%" source="images/FourierEx1.png" >
          <shortdescription></shortdescription>
        </image>
      </statement>
    </example>

    <problem>

      <idx><h>Fourier Series</h><h>sine series of an odd function</h></idx>

      <statement>
        <p>
          Let <m>n</m> be a positive integer.
          Show that if
          <me>
            f(x)=\frac{1}{2}-\abs{x-\frac{1}{2}}
          </me>
          then
          <me>
            \int_{x=0}^1f(x)\sin\left(n\pi x\right)d x = \frac{2}{\left(n\pi\right)^2}\sin\left(\frac{n\pi}{2}\right)
          </me>
          and show that the Fourier sine series of <m>f</m> is given by

          <md>
            <mrow>
              f(x)\amp{}=\sum_{n=1}^\infty\frac{4}{\left(n\pi\right)^2}\sin\left(\frac{n\pi}{2}
              \right)\sin\left(n\pi x\right)
            </mrow>
            <mrow>
              \amp{}=\frac{4}{\pi^2}\sum_{k=0}^\infty\frac{\left(-1\right)^k}{\left(2k+1\right)^2}\sin\left(\left(2k+1\right)\pi x\right).{}
            </mrow>
          </md>
        </p>
      </statement>
    </problem>

    <p>
      To see evidence that this series really does, in fact, represent
      <m>f</m> on <m>[0,1]</m>, let
      <me>
        S_N(x)=\frac{4}{\pi^2}\sum_{k=0}^N\frac{\left(-1\right)^k}{\left(2k+1\right)^2} \sin\left(\left(2k+1\right)\pi x\right)
      </me>
      be the <m>Nth</m> partial sum of the series.
      <!-- </p> -->

      <!-- <p> -->
      <!--   That is, <m>S_N</m> denotes the <m>N^{th}</m> partial sum of the -->
      <!--   series. --> 
      The sketches below display the graphs of <m>S_N</m> when
    <m>N=1</m>, <m>N=2</m>, <m>N=5</m>, and <m>N=50</m>.
  </p>
  <!-- <aside> -->
  <!--   <title>Note to self</title> -->
  <!--   <p> -->
  <!--     Need to find a way to make all of these graphs live and interactive. -->
  <!--   </p> -->
  <!-- </aside> -->

  <sbsgroup widths="45% 45%" margins="auto" valign="middle">
    <sidebyside>
      <figure>
        <caption>
          Graph of <m>S_1(x)</m>
        </caption>
        <image width="75%" source="images/FourierEx2-1.png" />
      </figure>
      <figure>
        <caption> 
          Graph of <m>S_2(x)</m>
        </caption>
        <image width="75%" source="images/FourierEx3-1.png" />
      </figure>
    </sidebyside>
    <sidebyside>
      <figure>
        <caption> 
          Graph of <m>S_5(x)</m>
        </caption>
        <image width="75%" source="images/FourierEx4-1.png" />
      </figure>
      <figure>
        <!-- <image width="75%" source="images/FourierEx5.png" /> -->
        <caption> 
          Graph of <m>S_{50}(x)</m>
        </caption>
        <image width="75%" source="images/FourierEx5-1.png" />
      </figure>

    </sidebyside>
  </sbsgroup>
  <!-- </p> -->
  <!-- <figure> -->
  <!-- <caption>The slider controls the number of terms in the partial sum. </caption> -->
  <!-- <interactive desmos="eru5fcn1ct" width="90%" aspect="2:1" preview="images/FourierEx4-1.png" /> -->
  <!-- <interactive desmos="eru5fcn1ct" width="90%" aspect="2:1"> --> 
  <!-- <interactive desmos="https://www.desmos.com/calculator/k3f5wcw8j6" width="90%" aspect="2:1"> -->
  <!-- <interactive desmos="jp8nvhadqk" width="125%" aspect="2:1"> -->
  <!-- <static> -->
  <!-- <caption></caption> -->
  <!-- <image source="images/FourierEx4.png"> -->
  <!-- <image width="75%" source="images/FourierEx2-1.png">  -->
  <!--   <shortdescription></shortdescription> -->
  <!-- </image> -->
  <!-- </static> -->
  <!-- </interactive> -->
  <!-- </figure> -->

  <p>
    As you can see, as we add more terms to <m>S_N</m> its graph looks
    more and more like the original function
    <m>f(x)=\frac{1}{2}-\abs{x-\frac{1}{2}}</m>.  This would seem to
    be strong evidence that series converges to the function and
    therefore
    <men xml:id="PDE_sol">
      f(x)=\frac{4}{\pi^2}\sum_{k=0}^\infty\frac{\left(-1\right)^k}{\left(2k+1\right)^2}\sin\left(\left(2k+1\right)\pi x\right)
      </men>.
      is a valid representation of <m>f</m> as a Fourier series.
  </p>
  <p>
    But is it?
  </p>
<p>
  Recall, that when we represented a function as a power series,
  we freely differentiated and integrated the series term by term as though it was a polynomial.
  Let<rsq/>s do the same with this Fourier series.
</p>

<p>
  To start, notice that the derivative of
  <me>
    f(x)=\frac{1}{2}-\abs{x-\frac{1}{2}}
  </me>
  is given by
  <me>
    f^\prime(x) = \begin{cases}1\amp \text{ if } \,\text{ } 0\leq x\lt \frac{1}{2}\\ -1\amp \text{ if } \,\frac{1}{2}\lt x\leq 1 \end{cases} 
    </me>.
</p>

<p>
  This derivative does not exist at
  <m>x=\frac{1}{2}</m> and its graph is given by  
</p>
<figure>
  <caption>
    Graph of 
    <m>
      f^\prime(x) = 
      \begin{cases}
        1\amp \text{ if }  0\leq x\lt \frac{1}{2}\\ 
        -1\amp \text{ if } \frac{1}{2}\lt x\leq 1 
      \end{cases} 
    </m>
  </caption>
  <image width="75%" source="images/Ch2fig1-1.png" >
    <shortdescription></shortdescription>
  </image>
</figure>
<p>
  If we differentiate the Fourier series in <xref ref="PDE_sol"
  >equation</xref> term<ndash/>by<ndash/>term, we obtain
  <men xml:id="EQUATIONPDESolDeriv">
    \frac{4}{\pi}\sum_{k=0}^\infty\frac{\left(-1\right)^k}{\left(2k+1\right)}
    \cos\left(\left(2k+1\right)\pi x\right) 
    </men>.
    Let
    <m>C_N(x)=\frac{4}{\pi}\sum_{k=0}^N\frac{\left(-1\right)^k}{\left(2k+1\right)}
    \cos\left(\left(2k+1\right)\pi x\right)</m> be the <m>Nth</m>
    partial sum of this Fourier cosine series.
    The sketches below display the graphs of <m>C_N</m> when
    <m>N=1</m>, <m>N=2</m>, <m>N=5</m>, and <m>N=50</m>.
</p>
<sbsgroup widths="45% 45%" margins="auto" valign="middle">
  <sidebyside>

    <figure >
      <caption>Graph of <m>C_1(x)</m></caption>
      <image width="75%" source="images/FourierEx6-1.png" />
    </figure>

    <figure >
      <caption>Graph of <m>C_1(x)</m></caption>
      <image width="75%" source="images/FourierEx7-1.png" />
    </figure>
  </sidebyside>
  <sidebyside>
    <figure >
      <caption>Graph of <m>C_5(x)</m></caption>
      <image width="75%" source="images/FourierEx8-1.png" />
    </figure>
    <figure >
      <caption>Graph of <m>C_{50}(x)</m></caption>
      <image width="75%" source="images/FourierEx9-1.png" />
    </figure>
  </sidebyside>
</sbsgroup>
<!--   <figure> -->
<!--     <!-\- <caption>The slider controls the number of terms being. .</caption> -\-> -->
<!--     <interactive desmos="0qatde8f0w" width="125%" aspect="2:1" >   -->
<!-- <static> -->
<!-- <figure > -->
<!--   <caption>Graph of <m>C_1(x)</m></caption> -->
<!--   <image width="75%" source="images/FourierEx8.png"> -->
<!--     <shortdescription></shortdescription> -->
<!--   </image> -->
<!-- </figure> -->
<!-- </static> -->
<!--     </interactive> -->
<!--   </figure> -->


<p>
  In fact, if we were to graph the series
  <m>\frac{4}{\pi}\sum_{k=0}^\infty\frac{\left(-1\right)^k}{\left(2k+1\right)}</m> cos<m>\left(\left(2k+1\right)\pi x\right)</m>,
  we would obtain the following graph:
</p>

<figure >
  <caption></caption>
  <image source="images/FourierEx10-1.png" width="75%">
    <shortdescription></shortdescription>
  </image>
</figure>

<!-- <sidebyside widths="90%" margins="auto" valign="middle"> -->
<!--   <image width="75%" source="images/FourierEx10.png" /> -->
<!-- </sidebyside> -->

<p>
  Notice that this agrees with the graph of <m>f^\prime</m>, except
  that <m>f^\prime</m> didn<rsq/>t exist at <m>x=\frac{1}{2}</m>, and
  this series takes on the value <m>0</m> at <m>x=\frac{1}{2}</m>.
  Notice also, that every partial sum of this series is continuous,
  since it is a finite combination of continuous cosine functions.
  This agrees with what you learned in Calculus, the (finite) sum of
  continuous functions is always continuous.  In the 1700s it was
  assumed (falsely) that this could be extended to infinite series,
  because every time a power series converged to a function, that
  function happened to be continuous.  This never failed for power
  series, so this example was a bit disconcerting as it is an example
  of the sum of infinitely many continuous functions which is, in this
  case, discontinuous.  Was it possible that there was some power
  series which converged to a function which was not continuous?  Even
  if there isn<rsq/>t, what is the difference between power series and
  this Fourier series?
</p>

<p>
  Even more disconcerting is what happens if we  differentiate the series

  <me>
    \frac{4}{\pi}\sum_{k=0}^\infty\frac{\left(-1\right)^k}{\left(2k+1\right)} \cos\left(\left(2k+1\right)\pi x\right)
  </me>

  term<ndash/>by<ndash/>term as before.  Given the above graph of this
  series, it appears that the derivative of it should be constantly 0,
  except at <m>x=\frac{1}{2}</m>, where the derivative doesn<rsq/>t exist.
  But when we perform the differentiation term<ndash/>by<ndash/>term
  we obtain the series
  <me>
    4\sum_{k=0}^\infty\left(-1\right)^{k+1}\sin\left(\left(2k+1\right)\pi x\right)
    </me>.
    and 
    if we graph the  sum of  the first forty terms of this series,
    we get: 
    
    <!-- <figure> -->
    <!-- <caption>The slider controls the number of terms being. .</caption> -->
    <!--     <interactive desmos="pvcgqtqso6" width="125%" aspect="2:1" > -->
    <!-- <static> -->
    <!-- <image source="images/FourierEx11.png"> -->
    <!-- </image> -->
    <!-- </static> -->
    <!--     </interactive> -->
    <!--   </figure> -->

</p>
    <image width="75%" source="images/FourierEx11-1.png" >
      <shortdescription></shortdescription>
    </image>
    <p>
      We knew that there might be a problem at <m>x=\frac{1}{2}</m> but this is crazy!
      The series doesn<rsq/>t seem to be converging to zero at all!
    </p>

    <problem xml:id="prob_FourierDiverge">

      <idx><h>Fourier Series</h></idx>
      <idx><h>Fourier Series</h><h>divergent Fourier series example</h></idx>

      <statement>
        <p>
          Show that when <m>x=\frac{1}{4}</m>

          <md>
            <mrow>
              4\sum_{k=0}^\infty\left(-1\right)^{k+1}\amp{} \sin\left(\left(2k+1\right)\pi x\right)
            </mrow>
            <mrow>
              \amp{}=4\left(-\frac{1}{\sqrt{2}}+\frac{1}{\sqrt{2}}+\frac{1}{\sqrt{2}}- \frac{1}{\sqrt{2}}-\frac{1}{\sqrt{2}}+\cdots\right).
            </mrow>

          </md>
        </p>
      </statement>
    </problem>

    <p>
      <xref ref="prob_FourierDiverge"></xref>
      shows that when we differentiate the series
      <me>
        \frac{4}{\pi}\sum_{k=0}^\infty\frac{\left(-1\right)^k}{\left(2k+1\right)} \cos\left(\left(2k+1\right)\pi x\right)
      </me>
      term by term,
      this differentiated series doesn<rsq/>t converge to anything at <m>x=\frac{1}{4}</m>,
      let alone converge to zero.
      In this case,
      the old Calculus rule that the derivative of a sum is the sum of the derivatives does not apply for this infinite sum,
      though it did apply before.
      As if the continuity issue wasn<rsq/>t bad enough before, this was even worse.
      Power series were routinely differentiated and integrated term-by-term.
      This was part of their appeal.
      They were treated like <q>infinite polynomials.</q>
      Either there is some power series lurking that refuses to behave nicely,
      or there is some property that power series have that not all Fourier series have. 
    </p>
    <p>
      Could it be that everything we did in <xref ref="CalcIn17th18thCentury" ></xref> and <xref
      ref="PowerSeriesQuestions"></xref> was bogus?
    </p>


    <p>
      Fortunately, the answer to that question is, <q>No.</q> Power
      series are generally much more well<ndash/>behaved than
      Fourier series.  Whenever a power series converges, the
      function it converges to will be continuous.  And, as long as
      one stays inside the interval of convergence, power series can
      be differentiated and integrated term<ndash/>by<ndash/>term.
      Power series have something going for them that your average
      Fourier series does not, but none of this is any more obvious
      to us than it was to mathematicians at the beginning of the
      nineteenth century.  What they did (and we do) know was that
      relying on intuition was perilous and that rigorous
      formulations were needed to either justify or dismiss these
      intuitions.  In some sense, the nineteenth century was the
      <q>morning after</q> the mathematical party that went on
      throughout the eighteenth century.
    </p>

    <aside>
      <title>
        Convergence: Power Series vs. Fourier Series
      </title>

      <p>
        We will prove all of these assertions in <xref ref="PowerSeriesRedux" ></xref>.
      </p>
    </aside>


    <problem xml:id="prob_Fourier_Series-orthogonality">
      
      <idx><h><m>\cos (nx)</m></h><h>orthogonality of</h></idx>
      <idx><h>orthogonality</h><h> of <m>\cos nx</m></h></idx>

      <statement>
        <p>
          Let <m>n</m> and <m>m</m> be positive integers.
          Show
          <me>
            \int_{x=0}^1\cos\left(n\pi x\right)\cos\left(m\pi x\right)\dx{ x}=\left\{ \begin{matrix}0\amp \text{ if } n\neq m\\ \frac{1}{2}\amp \text{ if } n=m \end{matrix} \right.
            </me>.
        </p>
      </statement>
    </problem>

        <problem xml:id="prob_fouriercoef">

          <idx><h>Fourier Series</h><h>computing the coefficients</h></idx>

          <statement>
          <p>
            Use the result of <xref ref="prob_Fourier_Series-orthogonality"></xref> to show that if
            <me>
              f(x)=\sum_{n=1}^\infty B_n\cos\left(n\pi x\right)
            </me>
            on <m>[0,1]</m>, then
            <men xml:id="EQUATIONCosineCoeffFourier">
              B_m=2\int_{x=0}^1f(x)\cos\left(m\pi x\right)\dx{ x}.{}
            </men>
          </p>
          </statement>
        </problem>

        <problem>
          
          <idx><h>Fourier Series</h><h>cosine series</h><h>the Fourier cosine series of <m>f(x)=x-\frac{1}{2}</m></h></idx>
          <statement>
            <p>
              Apply the result of <xref
              ref="prob_fouriercoef"></xref> to show that the Fourier
              cosine series of <m>f(x)=x-\frac{1}{2}</m> on <m>[0,1]</m> is
              given by
              <me>
                \frac{-4}{\pi^2}\sum_{k=0}^\infty\frac{1}{\left(2k+1\right)^2}\cos \left((2k+1)\pi x\right)
                </me>.
              </p>

              <p>
                Let 
                <me>
                  C(x,N)=\frac{-4}{\pi^2}\sum_{k=0}^N\frac{1}{\left(2k+1\right)^2}\cos
                  \left((2k+1)\pi x\right)
                </me>
                and plot <m>C(x,N)</m> for <m>N=1,2,5,50</m> <m>x\in[\,0,1]</m>.
                How does this compare to the function <m>f(x)=x-\frac{1}{2}</m> on <m>[\,0,1]</m>?
                What if you plot it for <m>x\in[\,0,2]?</m>
              </p>
            </statement>
          </problem>

          <problem>
            
            <idx><h>Fourier Series</h><h>term by term differentiation of</h></idx>

            <task>
              <statement>
                <p>
                  Differentiate the series
                  <me>
                    \frac{-4}{\pi^2}\sum_{k=0}^\infty\frac{1}{\left(2k+1\right)^2}\cos \left((2k+1)\pi x\right)
</me>
term by term and plot various partial sums for that series
on <m>[\,0,1]</m>.  How does this compare to the derivative
of <m>f(x)=x-\frac{1}{2}</m> on that interval?
</p>
</statement>
</task>
<task>
  <statement>
    <p>
      Differentiate the series you obtained in part (a) and plot
      various partial sums of that on <m>[\,0,1]</m>.  How does
      this compare to the second derivative of
      <m>f(x)=x-\frac{1}{2}</m> on that interval?
</p>
</statement>
</task>
</problem>

</section>
</chapter>
